proof/examples/zk/W64_exp_proof_5.ec
@@ -21,10 +21,10 @@ module M5 = {
 
     proc expm' (x:W64.t, n:W64.t) : W64.t = {
     
-    var x1, x2, x3, x4, bit, d, p, par : W64.t;
-    var ctr:int;
+    var x1, x2, x3, x4, bit, d, p, par, t1, t2 : W64.t;
+    var ctr: int;
 
-    d <- ith_bitword64 n (W64.size - 1);
+    d <@ ASpecFp.ith_bit(n,  (W64.size - 1));
     (x1,x2,x3) <- (W64.one,W64.one,x);
     x4 <@ ASpecFp.mulmw64(x,x);
 
@@ -36,24 +36,27 @@ module M5 = {
     while (0 < ctr) {
       ctr <- (ctr - 1);
       p <- d;
-      d <-  d `|` ith_bitword64 n ctr;
-      par <- ith_bitword64 n (ctr + 1) `^` ith_bitword64 n ctr;
+      t1 <@ ASpecFp.ith_bit(n,  (ctr + 1));
+      t2 <@ ASpecFp.ith_bit(n, ctr);
+      d <-  d `|` t2;
+      par <- t1 `^` t2;
       (x1,x2) <- if as_bool par then (x2,x1) else (x1, x2);
       x1 <@ ASpecFp.mulmw64(x1,x2); 
       x2 <@ ASpecFp.mulmw64(x2,x2);  
       (x1,x3) <- as_bool (d `^` p) ? (x3,x1) : (x1,x3);
       (x2,x4) <- as_bool (d `^` p)  ? (x4,x2) : (x2,x4);
     }
-    (x1,x2) <- if ! as_bool (ith_bitword64 n 0)  then (x2,x1) else (x1, x2);    
+    par <@ ASpecFp.ith_bit(n,0);
+    (x1,x2) <- if ! as_bool par  then (x2,x1) else (x1, x2);    
     return x1;
   }  
 
     proc expm (m : W64.t, x:W64.t, n:W64.t) : W64.t = {
     
-    var x1, x2, x3, x4, bit, d, p, par : W64.t;
+    var x1, x2, x3, x4, bit, d, p, par, t1, t2 : W64.t;
     var ctr:int;
 
-    d <- ith_bitword64 n (W64.size - 1);
+    d <@ M.__ith_bit64(n,  W64.of_int (W64.size - 1));
     (x1,x2,x3) <- (W64.one,W64.one,x);
     x4 <@ M.mulm(m,x,x);
 
@@ -65,15 +68,18 @@ module M5 = {
     while (0 < ctr) {
       ctr <- (ctr - 1);
       p <- d;
-      d <-  d `|` ith_bitword64 n ctr;
-      par <- ith_bitword64 n (ctr + 1) `^` ith_bitword64 n ctr;
+      t1 <@ M.__ith_bit64(n, W64.of_int (ctr + 1));
+      t2 <@ M.__ith_bit64(n, W64.of_int ctr);
+      d <-  d `|` t2;
+      par <- t1 `^` t2;
       (x1,x2) <- if as_bool par then (x2,x1) else (x1, x2);
       x1 <@ M.mulm(m,x1,x2); 
       x2 <@ M.mulm(m,x2,x2);  
       (x1,x3) <- as_bool (d `^` p) ? (x3,x1) : (x1,x3);
       (x2,x4) <- as_bool (d `^` p)  ? (x4,x2) : (x2,x4);
     }
-    (x1,x2) <- if ! as_bool (ith_bitword64 n 0)  then (x2,x1) else (x1, x2);    
+    par <@ M.__ith_bit64(n,W64.of_int 0);
+    (x1,x2) <- if ! as_bool par  then (x2,x1) else (x1, x2);    
     return x1;
   }  
 
@@ -82,20 +88,72 @@ module M5 = {
 
 
 
+
 lemma exp_4_5' :
  equiv[ M4.expm ~ M5.expm'  : ={arg} ==> ={res}].
 proc.
 inline ASpecFp.mulmw64.
+inline ASpecFp.ith_bit.
     wp.
     wp.
-while (={ctr, n,  x1,x2,  x3, x4, d, p}).
+while (={ctr, n,  x1,x2,  x3, x4, d, p} ).
  wp. skip. progress. 
-wp.  
-skip. 
-progress.
+wp.  skip. progress. 
 qed.
 
 
+(* minu_one  twos_compl to_uint_and_mod*)
+
+lemma qqq x : 0 < x < 64 => W64.one.[x] = false.
+admit. (* progress. timeout 20. smt. *)
+qed.
+
+lemma exp_ithbit :
+ equiv[ M.__ith_bit64 ~ ASpecFp.ith_bit    : arg{2}.`1 = arg{1}.`1 /\  arg{2}.`2 = W64.to_uint arg{1}.`2 
+    /\ 0 <= ctr{2} < 64 ==> ={res}].
+    symmetry.
+proc. 
+wp. skip. 
+progress.
+rewrite /ith_bitword64.
+rewrite /as_word.
+rewrite /truncateu8.
+have -> : (to_uint (ctr{2} `&` (of_int 63)%W64))
+  = (to_uint ctr{2} %% 2 ^ 6).
+rewrite - to_uint_and_mod. auto.
+smt. simplify.
+have -> : (of_int (to_uint ctr{2} %% 64))%W8 = (of_int (to_uint ctr{2}))%W8.
+smt.
+rewrite /(`>>`).
+rewrite /(`>>>`).
+rewrite /W64.(`&`).
+rewrite /map2.
+case (k{2}.[to_uint ctr{2}]).
+progress.
+apply W64.ext_eq.
+progress.
+rewrite initiE. auto.
+simplify.
+rewrite initiE. auto.
+simplify.
+case (x = 0).
+progress. smt. 
+progress.
+have -> : W64.one.[x] = false. 
+smt (qqq).
+auto.
+progress.
+apply W64.ext_eq.
+progress.
+rewrite initiE. auto.
+simplify.
+rewrite initiE. auto.
+simplify.
+case (x = 0).
+progress. smt. 
+progress. 
+smt (qqq).
+qed.    
 
 
 lemma exp_4_5'' :
@@ -103,16 +161,21 @@ lemma exp_4_5'' :
 symmetry.
 proc. 
 wp. 
-while (={ctr, n,  x1,x2,  x3, x4, d, p} /\ ImplWord m{1} P).
+call exp_ithbit.
+while (={ctr, n,  x1,x2,  x3, x4, d, p} /\ ImplWord m{1} P /\  0 <= ctr{1} < 64).
  wp. 
 call mulm_specw64.
 call mulm_specw64. 
 wp. 
+call exp_ithbit.
+call exp_ithbit.
+wp.
 skip. 
-progress.
+progress. smt . smt. smt(). smt().
 wp. 
 call mulm_specw64. 
-wp. 
+wp.
+call exp_ithbit. 
 skip.
 progress.
 qed.
